src/Example2.v
@@ -1,0 +1,181 @@
+Require List.
+Import List.ListNotations.
+
+Require Import src.LambdaRef.
+
+(* map for Ref *)
+Definition e : Expr Empty_set := (
+  -\ -\ Ref (Var ($ None) <* ! Var None)
+).
+
+(* e typechecks *)
+Fact type_e (t1 t2 : type) :
+  T[ env_empty |- e ::: (t1 --> t2) --> (RefT t1) --> (RefT t2) ].
+Proof.
+  econstructor. econstructor. econstructor. econstructor.
+  Unshelve.
+  3:{ exact t1. }
+  all: repeat econstructor.
+Qed.
+
+(* map for Ref in place *)
+Definition e' : Expr Empty_set := (
+  -\ -\ Var None <- (Var ($ None) <* ! Var None)
+).
+
+(* e' typechecks *)
+Fact type_e' (t : type) :
+  T[ env_empty |- e' ::: (t --> t) --> (RefT t) --> Unit ].
+Proof.
+  econstructor. econstructor. econstructor.
+  Unshelve.
+  3:{ exact t. }
+  { econstructor. }
+  { econstructor.
+    Unshelve.
+    3:{ exact t. }
+    all: repeat econstructor.
+  }
+Qed.
+
+Definition e_id : Expr Empty_set := (
+  -\ Var None
+).
+
+(* e_id typechecks *)
+Fact type_e_id (t : type) :
+  T[ env_empty |- e_id ::: t --> t ].
+Proof.
+  econstructor. econstructor.
+Qed.
+
+Definition e_ref_u : Expr Empty_set := (
+  Ref U_val
+).
+
+(* e_ref_u typechecks *)
+Fact type_e_ref_u : T[ env_empty |- e_ref_u ::: RefT Unit ].
+Proof.
+  econstructor. econstructor.
+Qed.
+
+(* -------------------------------------------------------- *)
+
+Definition ex : Expr Empty_set := e <* e_id <* e_ref_u.
+
+Fact type_ex : T[ env_empty |- ex ::: RefT Unit ].
+Proof.
+  econstructor.
+  { econstructor.
+    { apply type_e. }
+    { apply type_e_id. }
+  }
+  { apply type_e_ref_u. }
+Qed.
+
+Goal exists l m c,
+  cost_red ex []%list (Lab l) m c /\
+  List.In (l, U_val) m.
+Proof.
+  eexists. eexists. eexists. constructor.
+  { econstructor.
+    { econstructor. econstructor. }
+    { cbn. econstructor.
+      { apply red_app2. econstructor. unfold Is_fresh_label.
+        simpl. easy.
+      }
+      { econstructor.
+        { econstructor. }
+        { cbn. econstructor.
+          { econstructor. apply red_app2. econstructor. econstructor. }
+          { econstructor.
+            { econstructor. econstructor. }
+            { cbn. econstructor.
+              { econstructor. unfold Is_fresh_label. simpl. shelve. }
+              { econstructor. }
+            }
+          }
+        }
+      }
+    }
+  }
+  { econstructor. econstructor. }
+  Unshelve.
+  { constructor. exact 0. }
+  { constructor. exact 1. }
+  { intro H. destruct H as [H | []]. injection H. easy. }
+Qed.
+
+Definition ex' : Expr Empty_set := e' <* e_id <* e_ref_u.
+
+Fact type_ex' : T[ env_empty |- ex' ::: Unit ].
+Proof.
+  econstructor.
+  { econstructor.
+    { apply type_e'. }
+    { apply type_e_id. }
+  }
+  { apply type_e_ref_u. }
+Qed.
+
+Definition ex'' : Expr Empty_set :=
+  (-\ shift_e e' <* shift_e e_id <* Var None ;; Var None) <* e_ref_u.
+
+Fact type_ex'' : T[ env_empty |- ex'' ::: RefT Unit ].
+Proof.
+  econstructor.
+  { econstructor. econstructor.
+    { econstructor.
+      { econstructor.
+        { apply weakening. apply type_e'. }
+        { apply weakening. apply type_e_id. }
+      }
+      { shelve. }
+    }
+    { shelve. }
+  }
+  { apply type_e_ref_u. }
+  Unshelve.
+  { exact Unit. }
+  all: constructor.
+Qed.
+
+Goal exists l m c,
+  cost_red ex'' []%list (Lab l) m c /\
+  List.In (l, U_val) m.
+Proof.
+  eexists. eexists. eexists. constructor.
+  { econstructor.
+    { eapply red_app2. econstructor. unfold Is_fresh_label.
+      simpl. easy.
+    }
+    { cbn. econstructor.
+      { econstructor. }
+      { cbn. econstructor.
+        { econstructor. econstructor. econstructor. }
+        { cbn. econstructor.
+          { econstructor. econstructor. }
+          { cbn. econstructor.
+            { econstructor. apply red_assign2. apply red_app2.
+              econstructor. econstructor.
+            }
+            { econstructor.
+              { econstructor. apply red_assign2. econstructor. }
+              { econstructor.
+                { cbn. econstructor. econstructor. econstructor. }
+                { econstructor.
+                  { econstructor. }
+                  { econstructor. }
+                }
+              }
+            }
+          }
+        }
+      }
+    }
+  }
+  { constructor. constructor. }
+  Unshelve.
+  { constructor. exact 0. }
+  { exact []%list. }
+Qed.
